MMU_ARMv7_Refinement_No_Fault/ARMv7_Update_TTBR0_Ref.thy
@@ -309,24 +309,11 @@ lemma update_ttbr0_sat_no_flt_abs_refine':
 
 
 
-lemma  to_do':
-  "{v. (ASID s, v) \<in> ptable_comp (ASID s) (MEM s) (MEM s) (TTBR0 s) r} \<subseteq> 
-       snd ` ptable_comp (ASID s) (MEM s) (MEM s) (TTBR0 s) r"
-  apply (clarsimp simp: subset_image_iff)
-  apply (rule_tac x = "ptable_comp (ASID s) (MEM s) (MEM s) (TTBR0 s) r" in exI)
-  apply (rule conjI)
-   apply simp
-  apply (clarsimp simp: ptable_comp_def)
-  apply (clarsimp simp: snd_eq_Range)
-  by auto
-   
-
-
 lemma update_ttbr0_sat_no_flt_abs_refine'2:
-  "\<lbrakk> update_TTBR0 r (s::tlb_incon_state') = ((), s') ;  update_TTBR0 r (t::tlb_incon_state'2) = ((), t'); 
-             tlb_rel_abs'2 (typ_incon' s) (typ_incon'2 t) \<rbrakk> \<Longrightarrow> 
-                     tlb_rel_abs'2 (typ_incon' s') (typ_incon'2 t')"
-  apply (clarsimp simp: update_TTBR0_tlb_incon_state'2_ext_def update_TTBR0_tlb_incon_state'_ext_def tlb_rel_abs'2_def)
+  "\<lbrakk> update_TTBR0 r (s::tlb_incon_state') = ((), s') ;  update_TTBR0 r (t::tlb_incon_state) = ((), t'); 
+             refine_rel (typ_incon' s) (typ_incon'2 t) \<rbrakk> \<Longrightarrow> 
+                     refine_rel (typ_incon' s') (typ_incon'2 t')"
+  apply (clarsimp simp: update_TTBR0_tlb_incon_state_ext_def update_TTBR0_tlb_incon_state'_ext_def refine_rel_def)
   apply (subgoal_tac "ASID s = ASID t \<and> TTBR0 s = TTBR0 t \<and> MEM s = MEM t")
    prefer 2
    apply (clarsimp simp: typ_incon'2_def typ_incon'_def state.defs) 
@@ -334,28 +321,24 @@ lemma update_ttbr0_sat_no_flt_abs_refine'2:
    apply (clarsimp simp: typ_sat_no_flt_tlb_def "state.defs")
   apply (rule conjI)
    apply clarsimp
-
-
-
-
    apply (drule_tac x = a in spec)
-    apply (drule_tac x = a in spec)
-    apply clarsimp
-    apply (drule_tac x = v in spec)
-    apply (drule_tac x = v in spec)
-    apply rule  apply simp  
-    apply (erule disjE)
-     apply simp
-    apply (subgoal_tac "(a, v) \<notin> ptable_comp (ASID t) (MEM t) (MEM t) (TTBR0 t) r", simp)
-    apply (clarsimp simp: ptable_comp_def)
- apply (subgoal_tac  "{v. (ASID s, v) \<in> incon_set (tlb_incon_set' s) } \<subseteq> incon_set2 (tlb_incon_set'2 t)")
+   apply (drule_tac x = a in spec)
+   apply clarsimp
+   apply (drule_tac x = v in spec)
+   apply (drule_tac x = v in spec)
+   apply rule  apply simp  
+   apply (erule disjE)
+    apply simp
+   apply (subgoal_tac "(a, v) \<notin> ptable_comp (ASID t) (MEM t) (MEM t) (TTBR0 t) r", simp)
+   apply (clarsimp simp: ptable_comp_def)
+  apply (subgoal_tac  "{v. (ASID s, v) \<in> incon_set (tlb_incon_set' s) } \<subseteq> iset (tlb_incon_set t)")
    apply (subgoal_tac "{v. (ASID s, v) \<in> ptable_comp (ASID s) (MEM s) (MEM s) (TTBR0 s) r} \<subseteq> 
-           snd ` ptable_comp (ASID t) (MEM t) (MEM t) (TTBR0 t) r")
+            ptable_comp' (ASID t) (MEM t) (MEM t) (TTBR0 t) r")
     apply blast
-    prefer 2
-    apply clarsimp
-   by (clarsimp simp: to_do')
- 
+   prefer 2
+   apply clarsimp
+  by (clarsimp simp: ptable_comp_def ptable_comp'_def)
+
  
 
 end
